Examples/ArraySpec.v
@@ -13,25 +13,28 @@ From LHL.Util Require Import
   TransUtil
   Util.
 
+Definition Index N := {i | i < N}.
 
 Variant ArraySig {E} {N : nat} : ESig :=
-| At {A} (i : nat) (m : E A) : ArraySig A.
+| At {A} (i : Index N) (m : E A) : ArraySig A.
 Arguments ArraySig : clear implicits.
 
 Variant ArrayStep {T E N} {V : Spec T E} :
-  (nat -> State V) ->
+  (Index N -> State V) ->
   ThreadEvent T (ArraySig E N) ->
-  (nat -> State V) ->
+  (Index N -> State V) ->
   Prop :=
 | ArrayCall i A (m : E A) s t x y n :
-    n < N ->
+    (* n < N -> *)
+    True ->
     s n = x ->
     t n = y ->
     differ_pointwise s t n ->
     V.(Step) x (i, CallEv m) y ->
     ArrayStep s (i, CallEv (At n m)) t
 | ArrayRet i A (m : E A) v s t x y n :
-    n < N ->
+    (* n < N -> *)
+    True ->
     s n = x ->
     t n = y ->
     differ_pointwise s t n ->
@@ -40,9 +43,10 @@ Variant ArrayStep {T E N} {V : Spec T E} :
 Arguments ArrayStep {T E N} V.
 
 Program Definition arraySpec {T E} N (V : Spec T E) : Spec T (ArraySig E N) := {|
-  State := nat -> State V;
+  State := Index N -> State V;
   Step := ArrayStep V;
   Init _ := Init V
 |}.
 
-Admit Obligations.
+Next Obligation.
+Admitted.
