Examples/Array.v
@@ -1,0 +1,105 @@
+From LHL.Core Require Import
+  Program
+  Specs
+  Logic
+  LogicFacts
+  Tensor
+  Traces
+  SingConds
+  VisPoss
+  UBLayer
+  ProgramRules
+  Linearizability.
+
+From LHL.Util Require Import
+  TransUtil
+  Tactics
+  Util.
+
+From LHL.Examples Require Import
+  ArraySpec.
+
+Definition UnitSig : ESig :=
+    fun _ => Empty_set.
+
+Program Definition unitSpec {T} : Spec T UnitSig := {|
+  State := unit;
+  Step _ e _ := False;
+  Init := tt
+|}.
+
+Next Obligation.
+ddestruct H.
+constructor.
+easy.
+Qed.
+
+Fixpoint E (U : ESig) N :=
+  match N with
+  | 0 => UnitSig
+  | S N => U |+| E U N
+  end.
+
+Fixpoint VE {T U} (V : Spec T U) N : Spec T (E U N) :=
+  match N with
+  | 0 => unitSpec
+  | S N => tensorSpec V (VE V N)
+  end.
+
+Definition F U N := ArraySig U N.
+
+Definition VF {T U} (V : Spec T U) N : Spec T (F U N) :=
+  arraySpec N V.
+
+From Equations Require Import Equations.
+Require Import Lia.
+
+Equations getIndex {U N R} (i : Index N) (m : U R) : E U N R :=
+getIndex (N:= S N) (@exist _ _ 0 p) m := inl m;
+getIndex (N:= S N) (@exist _ _ (S i) p) m := inr (getIndex (@exist _ _ i _) m);
+getIndex (N:= 0) (@exist _ _ i p) m := _.
+
+Next Obligation. lia. Qed.
+Next Obligation. lia. Qed.
+
+Section indexVE.
+
+Context {T U} {V : Spec T U}.
+
+Equations indexVE {N} (i : Index N) (s : (VE V N).(State))
+  : V.(State) by wf (proj1_sig i) lt :=
+indexVE (N:= S N) (@exist _ _ 0 p) s := LState s;
+indexVE (N:= S N) (@exist _ _ (S i) p) s := indexVE (@exist _ _ i _) s;
+indexVE (N:= 0) (@exist _ _ i p) s := _.
+
+Next Obligation. lia. Qed.
+Next Obligation. lia. Qed.
+
+Definition index {U N R} (i : Index N) (m : U R) : Prog (E U N) R :=
+  Bind (getIndex i m)
+  Return.
+
+Definition arrayImpl {U N} : Impl (E U N) (ArraySig U N) :=
+  fun _ m => match m with
+  | At i m => index i m
+  end.
+
+Variant StRel {T U} {V : Spec T U} {N} :
+  ThreadState (E U N) (F U N) -> PCall (F U N) -> PRet (F U N) -> Prop :=
+| StIdle :
+  StRel Idle CallIdle RetIdle
+| StOCall i R (m : U R) :
+  StRel (Cont (At i m) (index i m)) (CallPoss (At i m)) RetIdle
+| StUCall i R (m : U R) :
+  StRel (UCall (At i m) (getIndex i m) Return) (CallDone (At i m)) RetIdle
+| StURet i R (m : U R) v :
+  StRel (Cont (At i m) (Return v)) (CallDone (At i m)) (RetPoss (At i m) v).
+
+Record Inv {T U} {V : Spec T U} {N}
+  (s : InterState (F U N) (VE V N)) (ρ : Poss (VF V N))
+:= {
+  st_cons : forall i, PState ρ i = indexVE i (snd s)
+}.
+
+Theorem arrayCorrect :
+  VerifyImpl
